Partial termination solution using decreases Repr

src/SDK/Keyring/Defs.dfy
@@ -9,7 +9,7 @@ module {:extern "KeyringDefs"} KeyringDefs {
   import Materials
   import AlgorithmSuite
 
-  trait {:termination false} {:extern} Keyring {
+  trait {:termination false} Keyring {
     ghost var Repr : set<object>
     predicate {:extern} Valid() reads this, Repr
 
@@ -26,6 +26,7 @@ module {:extern "KeyringDefs"} KeyringDefs {
       ensures res.Success? && res.value.Some? ==>
         var generateTraces: seq<Materials.KeyringTraceEntry> := Filter(res.value.get.keyringTrace, Materials.IsGenerateTraceEntry);
         |generateTraces| == if plaintextDataKey.None? then 1 else 0
+      decreases Repr
 
     method OnDecrypt(algorithmSuiteID: AlgorithmSuite.ID,
                      encryptionContext: Materials.EncryptionContext,
@@ -34,23 +35,70 @@ module {:extern "KeyringDefs"} KeyringDefs {
       ensures Valid()
       ensures |edks| == 0 ==> res.Success? && res.value.None?
       ensures res.Success? && res.value.Some? ==> res.value.get.algorithmSuiteID == algorithmSuiteID
+      decreases Repr
   }
 
   trait {:extern} ExternalKeyring {
+    ghost const Repr : set<object>
     method OnEncrypt(algorithmSuiteID: Materials.AlgorithmSuite.ID,
                      encryptionContext: Materials.EncryptionContext,
                      plaintextDataKey: Option<seq<uint8>>) returns (res: Result<Option<Materials.ValidDataKeyMaterials>>)
+        decreases Repr
 
     method OnDecrypt(algorithmSuiteID: AlgorithmSuite.ID,
                      encryptionContext: Materials.EncryptionContext,
                      edks: seq<Materials.EncryptedDataKey>) returns (res: Result<Option<Materials.ValidOnDecryptResult>>)
+        decreases Repr
   }
 
   class AsExternalKeyring extends ExternalKeyring {
     const wrapped: Keyring;
-
-    constructor(wrapped: Keyring) {
+    constructor(wrapped: Keyring) 
+        requires wrapped.Valid() 
+        ensures Valid() 
+        ensures fresh(Repr - {wrapped} - wrapped.Repr)
+    {
       this.wrapped := wrapped;
+      this.Repr := {this, wrapped} + wrapped.Repr;
+    }
+
+    predicate Valid() reads this, Repr {
+        && this in Repr 
+        && wrapped in Repr 
+        && wrapped.Repr <= Repr 
+        && this !in wrapped.Repr
+        && wrapped.Valid()
+    }
+
+    method OnEncrypt(algorithmSuiteID: Materials.AlgorithmSuite.ID,
+                     encryptionContext: Materials.EncryptionContext,
+                     plaintextDataKey: Option<seq<uint8>>) returns (res: Result<Option<Materials.ValidDataKeyMaterials>>) 
+      decreases Repr
+    {
+      var _ :- Require(Valid());
+      var _ :- Require(plaintextDataKey.Some? ==> algorithmSuiteID.ValidPlaintextDataKey(plaintextDataKey.get));
+      res := wrapped.OnEncrypt(algorithmSuiteID, encryptionContext, plaintextDataKey);
+    }
+
+    method OnDecrypt(algorithmSuiteID: AlgorithmSuite.ID,
+                     encryptionContext: Materials.EncryptionContext,
+                     edks: seq<Materials.EncryptedDataKey>) returns (res: Result<Option<Materials.ValidOnDecryptResult>>)
+      decreases Repr 
+    {
+      var _ :- Require(Valid());
+      res := wrapped.OnDecrypt(algorithmSuiteID, encryptionContext, edks);
+    }
+  }
+
+  class AsKeyring extends Keyring {
+    const wrapped: ExternalKeyring;
+
+    constructor(wrapped: ExternalKeyring) {
+      this.wrapped := wrapped;
+    }
+
+    predicate Valid() reads this, Repr {
+       true 
     }
 
     method OnEncrypt(algorithmSuiteID: Materials.AlgorithmSuite.ID,
@@ -63,38 +111,30 @@ module {:extern "KeyringDefs"} KeyringDefs {
       ensures res.Success? && res.value.Some? ==>
         var generateTraces: seq<Materials.KeyringTraceEntry> := Filter(res.value.get.keyringTrace, Materials.IsGenerateTraceEntry);
         |generateTraces| == if plaintextDataKey.None? then 1 else 0
+      decreases Repr
     {
       res := wrapped.OnEncrypt(algorithmSuiteID, encryptionContext, plaintextDataKey);
+      var _ :- Require(res.Success? && res.value.Some? ==> 
+          algorithmSuiteID == res.value.get.algorithmSuiteID);
+      var _ :- Require(res.Success? && res.value.Some? && plaintextDataKey.Some? ==> 
+          plaintextDataKey.get == res.value.get.plaintextDataKey);
+      var _ :- Require(res.Success? && res.value.Some? ==>
+        var generateTraces: seq<Materials.KeyringTraceEntry> := Filter(res.value.get.keyringTrace, Materials.IsGenerateTraceEntry);
+        |generateTraces| == if plaintextDataKey.None? then 1 else 0);
     }
 
     method OnDecrypt(algorithmSuiteID: AlgorithmSuite.ID,
                      encryptionContext: Materials.EncryptionContext,
-                     edks: seq<Materials.EncryptedDataKey>) returns (res: Result<Option<Materials.ValidOnDecryptResult>>) {
-      var _ :- Require(wrapped.Valid());
+                     edks: seq<Materials.EncryptedDataKey>) returns (res: Result<Option<Materials.ValidOnDecryptResult>>) 
+      ensures |edks| == 0 ==> res.Success? && res.value.None?
+      ensures res.Success? && res.value.Some? ==> res.value.get.algorithmSuiteID == algorithmSuiteID
+      decreases Repr
+    {
+      if |edks| == 0 {
+        return Success(None);
+      }
       res := wrapped.OnDecrypt(algorithmSuiteID, encryptionContext, edks);
-    }
-  }
-
-  class AsKeyring extends Keyring {
-    const wrapped: ExternalKeyring;
-
-    constructor(wrapped: ExternalKeyring) {
-      this.wrapped := wrapped;
-    }
-
-    predicate Valid() reads this, Repr { true }
-
-    method OnEncrypt(algorithmSuiteID: Materials.AlgorithmSuite.ID,
-                     encryptionContext: Materials.EncryptionContext,
-                     plaintextDataKey: Option<seq<uint8>>) returns (res: Result<Option<Materials.ValidDataKeyMaterials>>) {
-      var _ :- Require(plaintextDataKey.Some? ==> algorithmSuiteID.ValidPlaintextDataKey(plaintextDataKey.get));
-      res := wrapped.OnEncrypt(algorithmSuiteID, encryptionContext, plaintextDataKey);
-    }
-
-    method OnDecrypt(algorithmSuiteID: AlgorithmSuite.ID,
-                     encryptionContext: Materials.EncryptionContext,
-                     edks: seq<Materials.EncryptedDataKey>) returns (res: Result<Option<Materials.ValidOnDecryptResult>>) {
-      res := wrapped.OnDecrypt(algorithmSuiteID, encryptionContext, edks);
+      var _ :- Require(res.Success? && res.value.Some? ==> res.value.get.algorithmSuiteID == algorithmSuiteID);
     }
   }
 }
